Added syntax for lvalue expressions. Added example records

Example_Finite_Vars.thy
@@ -4,86 +4,77 @@ begin
 
 typedef mem = \<open>{f. \<forall>(n::string) (i::nat). f(n,i) \<in> {..i}}\<close>
   apply (rule exI[of _ \<open>\<lambda>_. 0\<close>]) by auto
+setup_lifting type_definition_mem
 
-definition var_raw0 :: "string \<Rightarrow> nat \<Rightarrow> (mem,nat) lvalue_raw" where
-  "var_raw0 n i = \<lparr> lv_domain = UNIV, lv_range = {..<i},
-    lv_getter = \<lambda>m. Rep_mem m (n,i-1),
-    lv_setter = \<lambda>a m. Abs_mem (fun_upd (Rep_mem m) (n,i-1) a) \<rparr>"
+definition idx_set where "idx_set (_::'a itself) = {..<CARD('a)}"
+definition some_f where "some_f = (SOME f. bij_betw f (idx_set TYPE('val)) (UNIV::'val::finite set))"
+definition some_f' :: "'val::finite\<Rightarrow>nat" where "some_f' = inv_into (idx_set TYPE('val)) some_f"
 
-lemma valid_var_raw0:
-  assumes "i \<noteq> 0"
-  shows "LValues.valid_lvalue (var_raw0 n i)"
-  unfolding var_raw0_def apply (rule valid_lvalueI)
-  using Rep_mem Rep_mem_inverse apply auto
-     apply (subst Abs_mem_inverse)
-      apply auto
-   apply (subst Abs_mem_inverse)
-    apply auto
-  by (metis Suc_le_lessD Suc_le_mono Suc_pred assms neq0_conv)
-
-lemma var_raw0_domain[simp]: "lv_domain (var_raw0 n i) = UNIV"
-  by (simp add: var_raw0_def)
-
-lemma var_raw0_range[simp]: "lv_range (var_raw0 n i) = {..<i}"
-  by (simp add: var_raw0_def)
-
-definition some_f where "some_f = (SOME f. bij_betw f {..<card (UNIV::'val::finite set)} (UNIV::'val set))"
-
-lemma bij_some_f: "bij_betw some_f {..<card (UNIV::'val::finite set)} (UNIV::'val set)"
-  unfolding some_f_def
-  apply (rule someI_ex[where P=\<open>\<lambda>f. bij_betw f {..<card (UNIV::'val set)} (UNIV::'val set)\<close>])
+lemma bij_some_f: "bij_betw some_f (idx_set TYPE('val)) (UNIV::'val::finite set)"
+  unfolding some_f_def 
+  apply (rule someI_ex[where P=\<open>\<lambda>f. bij_betw f (idx_set TYPE('val)) (UNIV::'val set)\<close>])
+  unfolding idx_set_def
   by (simp add: finite_same_card_bij)
 
-lemma inj_some_f: "inj_on (some_f::_\<Rightarrow>'val::finite) {..<card (UNIV::'val set)}"
-  using bij_betw_imp_inj_on bij_some_f by blast
+lemma bij_some_f': "bij_betw some_f' (UNIV::'val set) (idx_set TYPE('val::finite))"
+  by (simp add: bij_betw_inv_into bij_some_f some_f'_def)
 
-definition var_raw :: "string \<Rightarrow> (mem,'val::finite) lvalue_raw" where
-  "var_raw n = lvalue_map some_f
-     (var_raw0 n (card (UNIV::'val set)))"
+lemma some_f_some_f'[simp]: "some_f (some_f' x) = x"
+  by (metis UNIV_I bij_betw_inv_into_right bij_some_f some_f'_def)
 
-lemma valid_var_raw[simp]:
-  shows "LValues.valid_lvalue (var_raw n)"
-  unfolding var_raw_def
-  apply (rule valid_lvalue_map)
-   apply (rule valid_var_raw0, simp)
-  unfolding var_raw0_def
-  using inj_some_f by simp
+lemma some_f'_some_f[simp]: "x \<in> idx_set TYPE('val::finite) \<Longrightarrow> some_f' (some_f x :: 'val) = x"
+  unfolding some_f'_def
+  by (meson bij_betw_inv_into_left bij_some_f)
 
-lemma range_var_raw[simp]:
-  "lv_range (var_raw n) = UNIV"
-  unfolding var_raw_def apply simp
-  using bij_some_f
-  using bij_betw_imp_surj_on by blast
+lemma some_f'_leq: "some_f' (a::'a::finite) < CARD('a)"
+proof -
+  have "some_f' a \<in> idx_set TYPE('a)"
+    by (meson bij_betw_apply bij_some_f' iso_tuple_UNIV_I)
+  then show ?thesis
+    unfolding idx_set_def by auto
+qed
 
-lemma domain_var_raw[simp]:
-  "lv_domain (var_raw n) = UNIV"
-  unfolding var_raw_def by simp
+lift_definition var_getter :: "string \<Rightarrow> mem \<Rightarrow> 'a::finite" is
+  "\<lambda>name mem. some_f (mem (name, card (UNIV::'a set)-1))".
 
-lift_definition var :: "string \<Rightarrow> (mem,'val::finite) lvalue" is "Some o var_raw"
-  by auto
+lift_definition var_setter :: "string \<Rightarrow> 'a::finite \<Rightarrow> mem \<Rightarrow> mem" is
+  "\<lambda>name v mem. mem ((name, card (UNIV::'a set)-1) := some_f' v)"
+  using some_f'_leq less_Suc_eq_le by fastforce
 
-lemma valid_var[simp]: "valid_lvalue (var n)"
-  apply transfer by auto
+definition var :: "string \<Rightarrow> (mem,'a::finite) lvalue" where
+  "var name = mk_lvalue (var_getter name) (var_setter name)"
 
-lemma compatible_var_raw0:
-  assumes "n \<noteq> m" and "i \<noteq> 0" and "j \<noteq> 0"
-  shows "LValues.compatible_lvalues (var_raw0 n i) (var_raw0 m j)"
-  apply (rule compatible_lvalues.intros)
-     apply (auto simp: assms valid_var_raw0)
-  unfolding var_raw0_def apply (simp add: Rep_mem_inverse)
-  using Rep_mem apply (subst Abs_mem_inverse; auto)
-  using Rep_mem apply (subst Abs_mem_inverse; auto)
-  by (simp add: assms(1) fun_upd_twist)
+lemma valid_var[simp]: "valid_lvalue (var name :: (_,'val::finite) lvalue)"
+  unfolding var_def 
+proof (rule mk_lvalue_valid)
+  fix m and a b :: 'val
+  show "var_getter name (var_setter name a m) = a"
+    apply transfer by auto
+  show "var_setter name (var_getter name m) m = m"
+    apply transfer 
+    apply (subst some_f'_some_f) 
+    unfolding idx_set_def apply auto
+    by (metis Suc_le_lessD Suc_le_mono Suc_pred zero_less_card_finite)
+
+  show "var_setter name a (var_setter name b m) = var_setter name a m"
+    apply transfer by auto
+qed
+
+lemma var_setter_swap: 
+  assumes "name \<noteq> name'"
+  shows "var_setter name a (var_setter name' b m) = var_setter name' b (var_setter name a m)"
+  apply (transfer fixing: name name')
+  apply auto
+  using assms by auto
 
 lemma compatible_var: 
   "n \<noteq> m \<Longrightarrow> compatible_lvalues (var n) (var m)"
-  apply transfer apply simp
-  unfolding var_raw_def
-  apply (rule lvalue_map_compat1)
-  apply (rule lvalue_map_compat2)
+  unfolding var_def
+  apply (rule mk_lvalue_compat)
+  using valid_var unfolding var_def
   apply auto
-    apply (rule compatible_var_raw0)
-  using inj_some_f by auto
+  apply (subst var_setter_swap)
+  by auto
 
 definition x::"(mem,bool)lvalue" where "x = var ''x''"
 definition y::"(mem,32 word)lvalue" where "y = var ''y''"
@@ -99,8 +90,6 @@ lemma compat_xy[simp]: "compatible_lvalues x y"
 
 lemma compat_yx[simp]: "compatible_lvalues y x"
   by (simp add: compatible_var x_def y_def)
-
-
 
 lemma test:
   "getter (lvalue_pair x y) (setter x True (setter y 99 m))
